Do.lean
@@ -1,5 +1,6 @@
+-- This module serves as the root of the `Do` library.
+-- Import modules here that should be built as part of the library.
 import Do.Basic
 import Do.Mut
-import Do.Return
 import Do.For
 import Do.Formal
