lakefile.lean
@@ -1,9 +1,0 @@
-import Lake
-open Lake DSL
-
-package «do»
-
-@[defaultTarget]
-lean_lib Do
-
-require aesop from git "https://github.com/JLimperg/aesop.git"
